Adding rules for intptr casts + examples.
Co-authored-by: Michael Sammler <msammler@mpi-sws.org>

examples/intptr.c
@@ -1,0 +1,52 @@
+#include <refinedc.h>
+#include <stddef.h>
+
+[[rc::args("&own<int<i32>>")]]
+[[rc::returns("int<size_t>")]]
+size_t int_ptr(int* p){
+  size_t i = (size_t) p;
+  return i;
+}
+
+[[rc::parameters("p1 : loc", "p2 : loc")]]
+[[rc::args("p1 @ &own<int<i32>>", "p2 @ &own<int<i32>>")]]
+[[rc::returns("{p1.2 `min` p2.2} @ int<size_t>")]]
+size_t min_ptr_val(int *p1, int *p2){
+  size_t i1 = (size_t) p1;
+  size_t i2 = (size_t) p2;
+
+  if(i1 <= i2){
+    return i1;
+  }
+
+  return i2;
+}
+
+[[rc::parameters("p : loc")]]
+[[rc::args("p @ &own<int<i32>>")]]
+[[rc::returns("{(None, p.2)} @ &own<singleton_place<{(None, p.2)}>>")]]
+int* roundtrip1(int* p){
+  size_t i = (size_t) p;
+  void *q = (void*) i;
+  return q;
+}
+
+[[rc::parameters("p : loc", "n : Z")]]
+[[rc::args("p @ &own<n @ int<i32>>")]]
+[[rc::returns("p @ &own<n @ int<i32>>")]]
+int* roundtrip2(int* p){
+  size_t i = (size_t) p;
+  int *q = (void*) i;
+  return rc_copy_alloc_id(q, p);
+}
+
+[[rc::parameters("p : loc", "n : Z")]]
+[[rc::args("p @ &own<n @ int<i32>>")]]
+[[rc::returns("n @ int<i32>")]]
+[[rc::ensures("p @ &own<n @ int<i32>>")]]
+int roundtrip_and_read(int* p){
+  size_t i = (size_t) p;
+  int *q = (int*) i;
+  int *r = rc_copy_alloc_id(q, p);
+  return *r;
+}
