examples/proofs/intptr/generated_spec.v
@@ -1,0 +1,35 @@
+From refinedc.typing Require Import typing.
+From refinedc.examples.intptr Require Import generated_code.
+Set Default Proof Using "Type".
+
+(* Generated from [examples/intptr.c]. *)
+Section spec.
+  Context `{!typeG Σ} `{!globalG Σ}.
+
+  (* Type definitions. *)
+
+  (* Specifications for function [int_ptr]. *)
+  Definition type_of_int_ptr :=
+    fn(∀ () : (); (&own (int (i32))); True)
+      → ∃ () : (), (int (size_t)); True.
+
+  (* Specifications for function [min_ptr_val]. *)
+  Definition type_of_min_ptr_val :=
+    fn(∀ (p1, p2) : loc * loc; (p1 @ (&own (int (i32)))), (p2 @ (&own (int (i32)))); True)
+      → ∃ () : (), ((p1.2 `min` p2.2) @ (int (size_t))); True.
+
+  (* Specifications for function [roundtrip1]. *)
+  Definition type_of_roundtrip1 :=
+    fn(∀ p : loc; (p @ (&own (int (i32)))); True)
+      → ∃ () : (), (((None, p.2)) @ (&own (singleton_place ((None, p.2))))); True.
+
+  (* Specifications for function [roundtrip2]. *)
+  Definition type_of_roundtrip2 :=
+    fn(∀ (p, n) : loc * Z; (p @ (&own (n @ (int (i32))))); True)
+      → ∃ () : (), (p @ (&own (n @ (int (i32))))); True.
+
+  (* Specifications for function [roundtrip_and_read]. *)
+  Definition type_of_roundtrip_and_read :=
+    fn(∀ (p, n) : loc * Z; (p @ (&own (n @ (int (i32))))); True)
+      → ∃ () : (), (n @ (int (i32))); (p ◁ₗ (n @ (int (i32)))).
+End spec.
